Setlec/Model/Extend.lean
@@ -4583,7 +4583,8 @@ theorem checkIndDecl_sound {env env₂ : Env} {block : List ConstantInfo}
             (cvC.levelParams = cvT.levelParams &&
               checkEtaThm env cvT.name cvC.name cvT.levelParams nP nF)
             cvC.name nP nF
-            (checkUnitThm env cvT.name cvT.levelParams nP) nP false) := by
+            (checkUnitThm env cvT.name cvT.levelParams nP) nP
+            (nF == 0 && piResultSort cvT.type == some Level.zero)) := by
       intro cv caps₂ hmem
       have hmemf : (ConstantInfo.indInfo cv caps₂) ∈
           ([ConstantInfo.indInfo cvT capsT] : List ConstantInfo) := by
